plugins/micromega/micromega.ml
@@ -157,11 +157,10 @@ module Coq_Pos =
        | XI q0 -> XO (add_carry p q0)
        | XO q0 -> XI (add p q0)
        | XH -> XO (succ p))
-    | XH ->
-      (match y with
-       | XI q0 -> XI (succ q0)
-       | XO q0 -> XO (succ q0)
-       | XH -> XI XH)
+    | XH -> (match y with
+             | XI q0 -> XI (succ q0)
+             | XO q0 -> XO (succ q0)
+             | XH -> XI XH)
 
   (** val pred_double : positive -> positive **)
 
@@ -456,10 +455,9 @@ module Z =
     | Zpos x' -> (match y with
                   | Zpos y' -> Coq_Pos.compare x' y'
                   | _ -> Gt)
-    | Zneg x' ->
-      (match y with
-       | Zneg y' -> compOpp (Coq_Pos.compare x' y')
-       | _ -> Lt)
+    | Zneg x' -> (match y with
+                  | Zneg y' -> compOpp (Coq_Pos.compare x' y')
+                  | _ -> Lt)
 
   (** val leb : z -> z -> bool **)
 
@@ -653,9 +651,7 @@ let mkPX cO ceqb p i q0 =
   | Pc c -> if ceqb c cO then mkPinj XH q0 else PX (p, i, q0)
   | Pinj (_, _) -> PX (p, i, q0)
   | PX (p', i', q') ->
-    if peq ceqb q' (p0 cO)
-    then PX (p', (Coq_Pos.add i' i), q0)
-    else PX (p, i, q0)
+    if peq ceqb q' (p0 cO) then PX (p', (Coq_Pos.add i' i), q0) else PX (p, i, q0)
 
 (** val mkXi : 'a1 -> 'a1 -> positive -> 'a1 pol **)
 
@@ -691,8 +687,8 @@ let rec psubC csub p c =
   | PX (p2, i, q0) -> PX (p2, i, (psubC csub q0 c))
 
 (** val paddI :
-    ('a1 -> 'a1 -> 'a1) -> ('a1 pol -> 'a1 pol -> 'a1 pol) -> 'a1 pol ->
-    positive -> 'a1 pol -> 'a1 pol **)
+    ('a1 -> 'a1 -> 'a1) -> ('a1 pol -> 'a1 pol -> 'a1 pol) -> 'a1 pol -> positive ->
+    'a1 pol -> 'a1 pol **)
 
 let rec paddI cadd pop q0 j = function
 | Pc c -> mkPinj j (paddC cadd q0 c)
@@ -708,8 +704,8 @@ let rec paddI cadd pop q0 j = function
    | XH -> PX (p2, i, (pop q' q0)))
 
 (** val psubI :
-    ('a1 -> 'a1 -> 'a1) -> ('a1 -> 'a1) -> ('a1 pol -> 'a1 pol -> 'a1 pol) ->
-    'a1 pol -> positive -> 'a1 pol -> 'a1 pol **)
+    ('a1 -> 'a1 -> 'a1) -> ('a1 -> 'a1) -> ('a1 pol -> 'a1 pol -> 'a1 pol) -> 'a1 pol
+    -> positive -> 'a1 pol -> 'a1 pol **)
 
 let rec psubI cadd copp pop q0 j = function
 | Pc c -> mkPinj j (paddC cadd (popp copp q0) c)
@@ -725,8 +721,8 @@ let rec psubI cadd copp pop q0 j = function
    | XH -> PX (p2, i, (pop q' q0)))
 
 (** val paddX :
-    'a1 -> ('a1 -> 'a1 -> bool) -> ('a1 pol -> 'a1 pol -> 'a1 pol) -> 'a1 pol
-    -> positive -> 'a1 pol -> 'a1 pol **)
+    'a1 -> ('a1 -> 'a1 -> bool) -> ('a1 pol -> 'a1 pol -> 'a1 pol) -> 'a1 pol ->
+    positive -> 'a1 pol -> 'a1 pol **)
 
 let rec paddX cO ceqb pop p' i' p = match p with
 | Pc _ -> PX (p', i', p)
@@ -742,8 +738,8 @@ let rec paddX cO ceqb pop p' i' p = match p with
    | Zneg k -> mkPX cO ceqb (paddX cO ceqb pop p' k p2) i q')
 
 (** val psubX :
-    'a1 -> ('a1 -> 'a1) -> ('a1 -> 'a1 -> bool) -> ('a1 pol -> 'a1 pol -> 'a1
-    pol) -> 'a1 pol -> positive -> 'a1 pol -> 'a1 pol **)
+    'a1 -> ('a1 -> 'a1) -> ('a1 -> 'a1 -> bool) -> ('a1 pol -> 'a1 pol -> 'a1 pol) ->
+    'a1 pol -> positive -> 'a1 pol -> 'a1 pol **)
 
 let rec psubX cO copp ceqb pop p' i' p = match p with
 | Pc _ -> PX ((popp copp p'), i', p)
@@ -759,8 +755,7 @@ let rec psubX cO copp ceqb pop p' i' p = match p with
    | Zneg k -> mkPX cO ceqb (psubX cO copp ceqb pop p' k p2) i q')
 
 (** val padd :
-    'a1 -> ('a1 -> 'a1 -> 'a1) -> ('a1 -> 'a1 -> bool) -> 'a1 pol -> 'a1 pol
-    -> 'a1 pol **)
+    'a1 -> ('a1 -> 'a1 -> 'a1) -> ('a1 -> 'a1 -> bool) -> 'a1 pol -> 'a1 pol -> 'a1 pol **)
 
 let rec padd cO cadd ceqb p = function
 | Pc c' -> paddC cadd p c'
@@ -772,13 +767,11 @@ let rec padd cO cadd ceqb p = function
      (match j with
       | XI j0 -> PX (p'0, i', (padd cO cadd ceqb (Pinj ((XO j0), q0)) q'))
       | XO j0 ->
-        PX (p'0, i',
-          (padd cO cadd ceqb (Pinj ((Coq_Pos.pred_double j0), q0)) q'))
+        PX (p'0, i', (padd cO cadd ceqb (Pinj ((Coq_Pos.pred_double j0), q0)) q'))
       | XH -> PX (p'0, i', (padd cO cadd ceqb q0 q')))
    | PX (p2, i, q0) ->
      (match Z.pos_sub i i' with
-      | Z0 ->
-        mkPX cO ceqb (padd cO cadd ceqb p2 p'0) i (padd cO cadd ceqb q0 q')
+      | Z0 -> mkPX cO ceqb (padd cO cadd ceqb p2 p'0) i (padd cO cadd ceqb q0 q')
       | Zpos k ->
         mkPX cO ceqb (padd cO cadd ceqb (PX (p2, k, (p0 cO))) p'0) i'
           (padd cO cadd ceqb q0 q')
@@ -787,8 +780,8 @@ let rec padd cO cadd ceqb p = function
           (padd cO cadd ceqb q0 q')))
 
 (** val psub :
-    'a1 -> ('a1 -> 'a1 -> 'a1) -> ('a1 -> 'a1 -> 'a1) -> ('a1 -> 'a1) -> ('a1
-    -> 'a1 -> bool) -> 'a1 pol -> 'a1 pol -> 'a1 pol **)
+    'a1 -> ('a1 -> 'a1 -> 'a1) -> ('a1 -> 'a1 -> 'a1) -> ('a1 -> 'a1) -> ('a1 -> 'a1
+    -> bool) -> 'a1 pol -> 'a1 pol -> 'a1 pol **)
 
 let rec psub cO cadd csub copp ceqb p = function
 | Pc c' -> psubC csub p c'
@@ -799,12 +792,10 @@ let rec psub cO cadd csub copp ceqb p = function
    | Pinj (j, q0) ->
      (match j with
       | XI j0 ->
-        PX ((popp copp p'0), i',
-          (psub cO cadd csub copp ceqb (Pinj ((XO j0), q0)) q'))
+        PX ((popp copp p'0), i', (psub cO cadd csub copp ceqb (Pinj ((XO j0), q0)) q'))
       | XO j0 ->
         PX ((popp copp p'0), i',
-          (psub cO cadd csub copp ceqb (Pinj ((Coq_Pos.pred_double j0), q0))
-            q'))
+          (psub cO cadd csub copp ceqb (Pinj ((Coq_Pos.pred_double j0), q0)) q'))
       | XH -> PX ((popp copp p'0), i', (psub cO cadd csub copp ceqb q0 q')))
    | PX (p2, i, q0) ->
      (match Z.pos_sub i i' with
@@ -812,16 +803,14 @@ let rec psub cO cadd csub copp ceqb p = function
         mkPX cO ceqb (psub cO cadd csub copp ceqb p2 p'0) i
           (psub cO cadd csub copp ceqb q0 q')
       | Zpos k ->
-        mkPX cO ceqb (psub cO cadd csub copp ceqb (PX (p2, k, (p0 cO))) p'0)
-          i' (psub cO cadd csub copp ceqb q0 q')
+        mkPX cO ceqb (psub cO cadd csub copp ceqb (PX (p2, k, (p0 cO))) p'0) i'
+          (psub cO cadd csub copp ceqb q0 q')
       | Zneg k ->
-        mkPX cO ceqb
-          (psubX cO copp ceqb (psub cO cadd csub copp ceqb) p'0 k p2) i
+        mkPX cO ceqb (psubX cO copp ceqb (psub cO cadd csub copp ceqb) p'0 k p2) i
           (psub cO cadd csub copp ceqb q0 q')))
 
 (** val pmulC_aux :
-    'a1 -> ('a1 -> 'a1 -> 'a1) -> ('a1 -> 'a1 -> bool) -> 'a1 pol -> 'a1 ->
-    'a1 pol **)
+    'a1 -> ('a1 -> 'a1 -> 'a1) -> ('a1 -> 'a1 -> bool) -> 'a1 pol -> 'a1 -> 'a1 pol **)
 
 let rec pmulC_aux cO cmul ceqb p c =
   match p with
@@ -831,17 +820,15 @@ let rec pmulC_aux cO cmul ceqb p c =
     mkPX cO ceqb (pmulC_aux cO cmul ceqb p2 c) i (pmulC_aux cO cmul ceqb q0 c)
 
 (** val pmulC :
-    'a1 -> 'a1 -> ('a1 -> 'a1 -> 'a1) -> ('a1 -> 'a1 -> bool) -> 'a1 pol ->
-    'a1 -> 'a1 pol **)
+    'a1 -> 'a1 -> ('a1 -> 'a1 -> 'a1) -> ('a1 -> 'a1 -> bool) -> 'a1 pol -> 'a1 -> 'a1
+    pol **)
 
 let pmulC cO cI cmul ceqb p c =
-  if ceqb c cO
-  then p0 cO
-  else if ceqb c cI then p else pmulC_aux cO cmul ceqb p c
+  if ceqb c cO then p0 cO else if ceqb c cI then p else pmulC_aux cO cmul ceqb p c
 
 (** val pmulI :
-    'a1 -> 'a1 -> ('a1 -> 'a1 -> 'a1) -> ('a1 -> 'a1 -> bool) -> ('a1 pol ->
-    'a1 pol -> 'a1 pol) -> 'a1 pol -> positive -> 'a1 pol -> 'a1 pol **)
+    'a1 -> 'a1 -> ('a1 -> 'a1 -> 'a1) -> ('a1 -> 'a1 -> bool) -> ('a1 pol -> 'a1 pol
+    -> 'a1 pol) -> 'a1 pol -> positive -> 'a1 pol -> 'a1 pol **)
 
 let rec pmulI cO cI cmul ceqb pmul0 q0 j = function
 | Pc c -> mkPinj j (pmulC cO cI cmul ceqb q0 c)
@@ -858,12 +845,11 @@ let rec pmulI cO cI cmul ceqb pmul0 q0 j = function
    | XO j' ->
      mkPX cO ceqb (pmulI cO cI cmul ceqb pmul0 q0 j p') i'
        (pmulI cO cI cmul ceqb pmul0 q0 (Coq_Pos.pred_double j') q')
-   | XH ->
-     mkPX cO ceqb (pmulI cO cI cmul ceqb pmul0 q0 XH p') i' (pmul0 q' q0))
+   | XH -> mkPX cO ceqb (pmulI cO cI cmul ceqb pmul0 q0 XH p') i' (pmul0 q' q0))
 
 (** val pmul :
-    'a1 -> 'a1 -> ('a1 -> 'a1 -> 'a1) -> ('a1 -> 'a1 -> 'a1) -> ('a1 -> 'a1
-    -> bool) -> 'a1 pol -> 'a1 pol -> 'a1 pol **)
+    'a1 -> 'a1 -> ('a1 -> 'a1 -> 'a1) -> ('a1 -> 'a1 -> 'a1) -> ('a1 -> 'a1 -> bool)
+    -> 'a1 pol -> 'a1 pol -> 'a1 pol **)
 
 let rec pmul cO cI cadd cmul ceqb p p'' = match p'' with
 | Pc c -> pmulC cO cI cmul ceqb p c
@@ -875,8 +861,7 @@ let rec pmul cO cI cadd cmul ceqb p p'' = match p'' with
      let qQ' =
        match j with
        | XI j0 -> pmul cO cI cadd cmul ceqb (Pinj ((XO j0), q0)) q'
-       | XO j0 ->
-         pmul cO cI cadd cmul ceqb (Pinj ((Coq_Pos.pred_double j0), q0)) q'
+       | XO j0 -> pmul cO cI cadd cmul ceqb (Pinj ((Coq_Pos.pred_double j0), q0)) q'
        | XH -> pmul cO cI cadd cmul ceqb q0 q'
      in
      mkPX cO ceqb (pmul cO cI cadd cmul ceqb p p') i' qQ'
@@ -886,20 +871,19 @@ let rec pmul cO cI cadd cmul ceqb p p'' = match p'' with
      let qP' = pmul cO cI cadd cmul ceqb (mkPinj XH q0) p' in
      let pP' = pmul cO cI cadd cmul ceqb p2 p' in
      padd cO cadd ceqb
-       (mkPX cO ceqb (padd cO cadd ceqb (mkPX cO ceqb pP' i (p0 cO)) qP') i'
-         (p0 cO)) (mkPX cO ceqb pQ' i qQ'))
+       (mkPX cO ceqb (padd cO cadd ceqb (mkPX cO ceqb pP' i (p0 cO)) qP') i' (p0 cO))
+       (mkPX cO ceqb pQ' i qQ'))
 
 (** val psquare :
-    'a1 -> 'a1 -> ('a1 -> 'a1 -> 'a1) -> ('a1 -> 'a1 -> 'a1) -> ('a1 -> 'a1
-    -> bool) -> 'a1 pol -> 'a1 pol **)
+    'a1 -> 'a1 -> ('a1 -> 'a1 -> 'a1) -> ('a1 -> 'a1 -> 'a1) -> ('a1 -> 'a1 -> bool)
+    -> 'a1 pol -> 'a1 pol **)
 
 let rec psquare cO cI cadd cmul ceqb = function
 | Pc c -> Pc (cmul c c)
 | Pinj (j, q0) -> Pinj (j, (psquare cO cI cadd cmul ceqb q0))
 | PX (p2, i, q0) ->
   let twoPQ =
-    pmul cO cI cadd cmul ceqb p2
-      (mkPinj XH (pmulC cO cI cmul ceqb q0 (cadd cI cI)))
+    pmul cO cI cadd cmul ceqb p2 (mkPinj XH (pmulC cO cI cmul ceqb q0 (cadd cI cI)))
   in
   let q2 = psquare cO cI cadd cmul ceqb q0 in
   let p3 = psquare cO cI cadd cmul ceqb p2 in
@@ -911,9 +895,8 @@ let mk_X cO cI j =
   mkPinj_pred j (mkX cO cI)
 
 (** val ppow_pos :
-    'a1 -> 'a1 -> ('a1 -> 'a1 -> 'a1) -> ('a1 -> 'a1 -> 'a1) -> ('a1 -> 'a1
-    -> bool) -> ('a1 pol -> 'a1 pol) -> 'a1 pol -> 'a1 pol -> positive -> 'a1
-    pol **)
+    'a1 -> 'a1 -> ('a1 -> 'a1 -> 'a1) -> ('a1 -> 'a1 -> 'a1) -> ('a1 -> 'a1 -> bool)
+    -> ('a1 pol -> 'a1 pol) -> 'a1 pol -> 'a1 pol -> positive -> 'a1 pol **)
 
 let rec ppow_pos cO cI cadd cmul ceqb subst_l res p = function
 | XI p3 ->
@@ -927,16 +910,16 @@ let rec ppow_pos cO cI cadd cmul ceqb subst_l res p = function
 | XH -> subst_l (pmul cO cI cadd cmul ceqb res p)
 
 (** val ppow_N :
-    'a1 -> 'a1 -> ('a1 -> 'a1 -> 'a1) -> ('a1 -> 'a1 -> 'a1) -> ('a1 -> 'a1
-    -> bool) -> ('a1 pol -> 'a1 pol) -> 'a1 pol -> n -> 'a1 pol **)
+    'a1 -> 'a1 -> ('a1 -> 'a1 -> 'a1) -> ('a1 -> 'a1 -> 'a1) -> ('a1 -> 'a1 -> bool)
+    -> ('a1 pol -> 'a1 pol) -> 'a1 pol -> n -> 'a1 pol **)
 
 let ppow_N cO cI cadd cmul ceqb subst_l p = function
 | N0 -> p1 cI
 | Npos p2 -> ppow_pos cO cI cadd cmul ceqb subst_l (p1 cI) p p2
 
 (** val norm_aux :
-    'a1 -> 'a1 -> ('a1 -> 'a1 -> 'a1) -> ('a1 -> 'a1 -> 'a1) -> ('a1 -> 'a1
-    -> 'a1) -> ('a1 -> 'a1) -> ('a1 -> 'a1 -> bool) -> 'a1 pExpr -> 'a1 pol **)
+    'a1 -> 'a1 -> ('a1 -> 'a1 -> 'a1) -> ('a1 -> 'a1 -> 'a1) -> ('a1 -> 'a1 -> 'a1) ->
+    ('a1 -> 'a1) -> ('a1 -> 'a1 -> bool) -> 'a1 pExpr -> 'a1 pol **)
 
 let rec norm_aux cO cI cadd cmul csub copp ceqb = function
 | PEc c -> Pc c
@@ -944,14 +927,12 @@ let rec norm_aux cO cI cadd cmul csub copp ceqb = function
 | PEadd (pe1, pe2) ->
   (match pe1 with
    | PEopp pe3 ->
-     psub cO cadd csub copp ceqb
-       (norm_aux cO cI cadd cmul csub copp ceqb pe2)
+     psub cO cadd csub copp ceqb (norm_aux cO cI cadd cmul csub copp ceqb pe2)
        (norm_aux cO cI cadd cmul csub copp ceqb pe3)
    | _ ->
      (match pe2 with
       | PEopp pe3 ->
-        psub cO cadd csub copp ceqb
-          (norm_aux cO cI cadd cmul csub copp ceqb pe1)
+        psub cO cadd csub copp ceqb (norm_aux cO cI cadd cmul csub copp ceqb pe1)
           (norm_aux cO cI cadd cmul csub copp ceqb pe3)
       | _ ->
         padd cO cadd ceqb (norm_aux cO cI cadd cmul csub copp ceqb pe1)
@@ -985,8 +966,8 @@ type ('tA, 'tX, 'aA, 'aF) gFormula =
 | EQ of ('tA, 'tX, 'aA, 'aF) gFormula * ('tA, 'tX, 'aA, 'aF) gFormula
 
 (** val mapX :
-    (kind -> 'a2 -> 'a2) -> kind -> ('a1, 'a2, 'a3, 'a4) gFormula -> ('a1,
-    'a2, 'a3, 'a4) gFormula **)
+    (kind -> 'a2 -> 'a2) -> kind -> ('a1, 'a2, 'a3, 'a4) gFormula -> ('a1, 'a2, 'a3,
+    'a4) gFormula **)
 
 let rec mapX f _ = function
 | X (k0, x) -> X (k0, (f k0 x))
@@ -1044,25 +1025,21 @@ type eKind = __
 type 'a bFormula = ('a, eKind, unit0, unit0) gFormula
 
 (** val map_bformula :
-    kind -> ('a1 -> 'a2) -> ('a1, 'a3, 'a4, 'a5) gFormula -> ('a2, 'a3, 'a4,
-    'a5) gFormula **)
+    kind -> ('a1 -> 'a2) -> ('a1, 'a3, 'a4, 'a5) gFormula -> ('a2, 'a3, 'a4, 'a5)
+    gFormula **)
 
 let rec map_bformula _ fct = function
 | TT k -> TT k
 | FF k -> FF k
 | X (k, p) -> X (k, p)
 | A (k, a, t0) -> A (k, (fct a), t0)
-| AND (k0, f1, f2) ->
-  AND (k0, (map_bformula k0 fct f1), (map_bformula k0 fct f2))
-| OR (k0, f1, f2) ->
-  OR (k0, (map_bformula k0 fct f1), (map_bformula k0 fct f2))
+| AND (k0, f1, f2) -> AND (k0, (map_bformula k0 fct f1), (map_bformula k0 fct f2))
+| OR (k0, f1, f2) -> OR (k0, (map_bformula k0 fct f1), (map_bformula k0 fct f2))
 | NOT (k0, f0) -> NOT (k0, (map_bformula k0 fct f0))
 | IMPL (k0, f1, a, f2) ->
   IMPL (k0, (map_bformula k0 fct f1), a, (map_bformula k0 fct f2))
-| IFF (k0, f1, f2) ->
-  IFF (k0, (map_bformula k0 fct f1), (map_bformula k0 fct f2))
-| EQ (f1, f2) ->
-  EQ ((map_bformula IsBool fct f1), (map_bformula IsBool fct f2))
+| IFF (k0, f1, f2) -> IFF (k0, (map_bformula k0 fct f1), (map_bformula k0 fct f2))
+| EQ (f1, f2) -> EQ ((map_bformula IsBool fct f1), (map_bformula IsBool fct f2))
 
 type ('x, 'annot) clause = ('x * 'annot) list
 
@@ -1079,8 +1056,8 @@ let cnf_ff =
   []::[]
 
 (** val add_term :
-    ('a1 -> bool) -> ('a1 -> 'a1 -> 'a1 option) -> ('a1 * 'a2) -> ('a1, 'a2)
-    clause -> ('a1, 'a2) clause option **)
+    ('a1 -> bool) -> ('a1 -> 'a1 -> 'a1 option) -> ('a1 * 'a2) -> ('a1, 'a2) clause ->
+    ('a1, 'a2) clause option **)
 
 let rec add_term unsat deduce t0 = function
 | [] ->
@@ -1101,8 +1078,8 @@ let rec add_term unsat deduce t0 = function
       | None -> None))
 
 (** val or_clause :
-    ('a1 -> bool) -> ('a1 -> 'a1 -> 'a1 option) -> ('a1, 'a2) clause -> ('a1,
-    'a2) clause -> ('a1, 'a2) clause option **)
+    ('a1 -> bool) -> ('a1 -> 'a1 -> 'a1 option) -> ('a1, 'a2) clause -> ('a1, 'a2)
+    clause -> ('a1, 'a2) clause option **)
 
 let rec or_clause unsat deduce cl1 cl2 =
   match cl1 with
@@ -1113,8 +1090,8 @@ let rec or_clause unsat deduce cl1 cl2 =
      | None -> None)
 
 (** val xor_clause_cnf :
-    ('a1 -> bool) -> ('a1 -> 'a1 -> 'a1 option) -> ('a1, 'a2) clause -> ('a1,
-    'a2) cnf -> ('a1, 'a2) cnf **)
+    ('a1 -> bool) -> ('a1 -> 'a1 -> 'a1 option) -> ('a1, 'a2) clause -> ('a1, 'a2) cnf
+    -> ('a1, 'a2) cnf **)
 
 let xor_clause_cnf unsat deduce t0 f =
   fold_left (fun acc e ->
@@ -1123,8 +1100,8 @@ let xor_clause_cnf unsat deduce t0 f =
     | None -> acc) f []
 
 (** val or_clause_cnf :
-    ('a1 -> bool) -> ('a1 -> 'a1 -> 'a1 option) -> ('a1, 'a2) clause -> ('a1,
-    'a2) cnf -> ('a1, 'a2) cnf **)
+    ('a1 -> bool) -> ('a1 -> 'a1 -> 'a1 option) -> ('a1, 'a2) clause -> ('a1, 'a2) cnf
+    -> ('a1, 'a2) cnf **)
 
 let or_clause_cnf unsat deduce t0 f =
   match t0 with
@@ -1132,14 +1109,13 @@ let or_clause_cnf unsat deduce t0 f =
   | _::_ -> xor_clause_cnf unsat deduce t0 f
 
 (** val or_cnf :
-    ('a1 -> bool) -> ('a1 -> 'a1 -> 'a1 option) -> ('a1, 'a2) cnf -> ('a1,
-    'a2) cnf -> ('a1, 'a2) cnf **)
+    ('a1 -> bool) -> ('a1 -> 'a1 -> 'a1 option) -> ('a1, 'a2) cnf -> ('a1, 'a2) cnf ->
+    ('a1, 'a2) cnf **)
 
 let rec or_cnf unsat deduce f f' =
   match f with
   | [] -> cnf_tt
-  | e::rst ->
-    rev_append (or_cnf unsat deduce rst f') (or_clause_cnf unsat deduce e f')
+  | e::rst -> rev_append (or_cnf unsat deduce rst f') (or_clause_cnf unsat deduce e f')
 
 (** val and_cnf : ('a1, 'a2) cnf -> ('a1, 'a2) cnf -> ('a1, 'a2) cnf **)
 
@@ -1173,8 +1149,8 @@ let and_cnf_opt f1 f2 =
   else if is_cnf_tt f2 then f1 else and_cnf f1 f2
 
 (** val or_cnf_opt :
-    ('a1 -> bool) -> ('a1 -> 'a1 -> 'a1 option) -> ('a1, 'a2) cnf -> ('a1,
-    'a2) cnf -> ('a1, 'a2) cnf **)
+    ('a1 -> bool) -> ('a1 -> 'a1 -> 'a1 option) -> ('a1, 'a2) cnf -> ('a1, 'a2) cnf ->
+    ('a1, 'a2) cnf **)
 
 let or_cnf_opt unsat deduce f1 f2 =
   if if is_cnf_tt f1 then true else is_cnf_tt f2
@@ -1182,9 +1158,9 @@ let or_cnf_opt unsat deduce f1 f2 =
   else if is_cnf_ff f2 then f1 else or_cnf unsat deduce f1 f2
 
 (** val mk_and :
-    ('a2 -> bool) -> ('a2 -> 'a2 -> 'a2 option) -> (bool -> kind -> ('a1,
-    'a3, 'a4, 'a5) tFormula -> ('a2, 'a3) cnf) -> kind -> bool -> ('a1, 'a3,
-    'a4, 'a5) tFormula -> ('a1, 'a3, 'a4, 'a5) tFormula -> ('a2, 'a3) cnf **)
+    ('a2 -> bool) -> ('a2 -> 'a2 -> 'a2 option) -> (bool -> kind -> ('a1, 'a3, 'a4,
+    'a5) tFormula -> ('a2, 'a3) cnf) -> kind -> bool -> ('a1, 'a3, 'a4, 'a5) tFormula
+    -> ('a1, 'a3, 'a4, 'a5) tFormula -> ('a2, 'a3) cnf **)
 
 let mk_and unsat deduce rEC k pol0 f1 f2 =
   if pol0
@@ -1192,9 +1168,9 @@ let mk_and unsat deduce rEC k pol0 f1 f2 =
   else or_cnf_opt unsat deduce (rEC pol0 k f1) (rEC pol0 k f2)
 
 (** val mk_or :
-    ('a2 -> bool) -> ('a2 -> 'a2 -> 'a2 option) -> (bool -> kind -> ('a1,
-    'a3, 'a4, 'a5) tFormula -> ('a2, 'a3) cnf) -> kind -> bool -> ('a1, 'a3,
-    'a4, 'a5) tFormula -> ('a1, 'a3, 'a4, 'a5) tFormula -> ('a2, 'a3) cnf **)
+    ('a2 -> bool) -> ('a2 -> 'a2 -> 'a2 option) -> (bool -> kind -> ('a1, 'a3, 'a4,
+    'a5) tFormula -> ('a2, 'a3) cnf) -> kind -> bool -> ('a1, 'a3, 'a4, 'a5) tFormula
+    -> ('a1, 'a3, 'a4, 'a5) tFormula -> ('a2, 'a3) cnf **)
 
 let mk_or unsat deduce rEC k pol0 f1 f2 =
   if pol0
@@ -1202,23 +1178,22 @@ let mk_or unsat deduce rEC k pol0 f1 f2 =
   else and_cnf_opt (rEC pol0 k f1) (rEC pol0 k f2)
 
 (** val mk_impl :
-    ('a2 -> bool) -> ('a2 -> 'a2 -> 'a2 option) -> (bool -> kind -> ('a1,
-    'a3, 'a4, 'a5) tFormula -> ('a2, 'a3) cnf) -> kind -> bool -> ('a1, 'a3,
-    'a4, 'a5) tFormula -> ('a1, 'a3, 'a4, 'a5) tFormula -> ('a2, 'a3) cnf **)
+    ('a2 -> bool) -> ('a2 -> 'a2 -> 'a2 option) -> (bool -> kind -> ('a1, 'a3, 'a4,
+    'a5) tFormula -> ('a2, 'a3) cnf) -> kind -> bool -> ('a1, 'a3, 'a4, 'a5) tFormula
+    -> ('a1, 'a3, 'a4, 'a5) tFormula -> ('a2, 'a3) cnf **)
 
 let mk_impl unsat deduce rEC k pol0 f1 f2 =
   if pol0
   then or_cnf_opt unsat deduce (rEC (negb pol0) k f1) (rEC pol0 k f2)
   else and_cnf_opt (rEC (negb pol0) k f1) (rEC pol0 k f2)
 
-(** val mk_iff :
-    ('a2 -> bool) -> ('a2 -> 'a2 -> 'a2 option) -> (bool -> kind -> ('a1,
-    'a3, 'a4, 'a5) tFormula -> ('a2, 'a3) cnf) -> kind -> bool -> ('a1, 'a3,
-    'a4, 'a5) tFormula -> ('a1, 'a3, 'a4, 'a5) tFormula -> ('a2, 'a3) cnf **)
+(** val mk_eq :
+    ('a2 -> bool) -> ('a2 -> 'a2 -> 'a2 option) -> (bool -> kind -> ('a1, 'a3, 'a4,
+    'a5) tFormula -> ('a2, 'a3) cnf) -> kind -> bool -> ('a1, 'a3, 'a4, 'a5) tFormula
+    -> ('a1, 'a3, 'a4, 'a5) tFormula -> ('a2, 'a3) cnf **)
 
-let mk_iff unsat deduce rEC k pol0 f1 f2 =
-  or_cnf_opt unsat deduce
-    (and_cnf_opt (rEC (negb pol0) k f1) (rEC false k f2))
+let mk_eq unsat deduce rEC k pol0 f1 f2 =
+  or_cnf_opt unsat deduce (and_cnf_opt (rEC (negb pol0) k f1) (rEC false k f2))
     (and_cnf_opt (rEC pol0 k f1) (rEC true k f2))
 
 (** val is_bool : kind -> ('a1, 'a2, 'a3, 'a4) tFormula -> bool option **)
@@ -1228,46 +1203,71 @@ let is_bool _ = function
 | FF _ -> Some false
 | _ -> None
 
+(** val is_FF : kind -> ('a1, 'a2, 'a3, 'a4) tFormula -> bool **)
+
+let is_FF _ = function
+| FF _ -> true
+| _ -> false
+
+(** val negate_formula :
+    kind -> ('a1, 'a2, 'a3, 'a4) tFormula -> ('a1, 'a3, 'a2, 'a4) gFormula **)
+
+let rec negate_formula _ = function
+| TT k0 -> FF k0
+| FF k0 -> TT k0
+| X (k0, _) -> TT k0
+| A (k0, _, _) -> TT k0
+| AND (k0, f1, f2) -> OR (k0, (negate_formula k0 f1), (negate_formula k0 f2))
+| OR (k0, f1, _) -> negate_formula k0 f1
+| NOT (_, e) -> e
+| IMPL (k0, f1, _, f2) ->
+  if is_FF k0 f2 then f1 else AND (k0, f1, (negate_formula k0 f2))
+| IFF (k0, _, _) -> TT k0
+| EQ (_, _) -> TT IsProp
+
 (** val xcnf :
-    ('a2 -> bool) -> ('a2 -> 'a2 -> 'a2 option) -> ('a1 -> 'a3 -> ('a2, 'a3)
-    cnf) -> ('a1 -> 'a3 -> ('a2, 'a3) cnf) -> bool -> kind -> ('a1, 'a3, 'a4,
+    ('a2 -> bool) -> ('a2 -> 'a2 -> 'a2 option) -> (kind -> 'a1 -> 'a3 -> ('a2, 'a3)
+    cnf) -> (kind -> 'a1 -> 'a3 -> ('a2, 'a3) cnf) -> bool -> kind -> ('a1, 'a3, 'a4,
     'a5) tFormula -> ('a2, 'a3) cnf **)
 
-let rec xcnf unsat deduce normalise1 negate0 pol0 _ = function
+let rec xcnf unsat deduce normalise1 negate0 pol0 k = function
 | TT _ -> if pol0 then cnf_tt else cnf_ff
 | FF _ -> if pol0 then cnf_ff else cnf_tt
 | X (_, _) -> cnf_ff
-| A (_, x, t0) -> if pol0 then normalise1 x t0 else negate0 x t0
+| A (_, x, t0) -> if pol0 then normalise1 k x t0 else negate0 k x t0
 | AND (k0, e1, e2) ->
-  mk_and unsat deduce (fun x x0 x1 ->
-    xcnf unsat deduce normalise1 negate0 x x0 x1) k0 pol0 e1 e2
+  mk_and unsat deduce (fun x x0 x1 -> xcnf unsat deduce normalise1 negate0 x x0 x1) k0
+    pol0 e1 e2
 | OR (k0, e1, e2) ->
-  mk_or unsat deduce (fun x x0 x1 ->
-    xcnf unsat deduce normalise1 negate0 x x0 x1) k0 pol0 e1 e2
+  mk_or unsat deduce (fun x x0 x1 -> xcnf unsat deduce normalise1 negate0 x x0 x1) k0
+    pol0 e1 e2
 | NOT (k0, e) -> xcnf unsat deduce normalise1 negate0 (negb pol0) k0 e
 | IMPL (k0, e1, _, e2) ->
-  mk_impl unsat deduce (fun x x0 x1 ->
-    xcnf unsat deduce normalise1 negate0 x x0 x1) k0 pol0 e1 e2
+  mk_impl unsat deduce (fun x x0 x1 -> xcnf unsat deduce normalise1 negate0 x x0 x1)
+    k0 pol0 e1 e2
 | IFF (k0, e1, e2) ->
-  (match is_bool k0 e2 with
-   | Some isb ->
-     xcnf unsat deduce normalise1 negate0 (if isb then pol0 else negb pol0)
-       k0 e1
-   | None ->
-     mk_iff unsat deduce (fun x x0 x1 ->
-       xcnf unsat deduce normalise1 negate0 x x0 x1) k0 pol0 e1 e2)
+  if pol0
+  then and_cnf_opt
+         (mk_impl unsat deduce (fun x x0 x1 ->
+           xcnf unsat deduce normalise1 negate0 x x0 x1) k0 pol0 e1 e2)
+         (mk_impl unsat deduce (fun x x0 x1 ->
+           xcnf unsat deduce normalise1 negate0 x x0 x1) k0 pol0 e2 e1)
+  else or_cnf_opt unsat deduce
+         (mk_impl unsat deduce (fun x x0 x1 ->
+           xcnf unsat deduce normalise1 negate0 x x0 x1) k0 pol0 e1 e2)
+         (mk_impl unsat deduce (fun x x0 x1 ->
+           xcnf unsat deduce normalise1 negate0 x x0 x1) k0 pol0 e2 e1)
 | EQ (e1, e2) ->
   (match is_bool IsBool e2 with
    | Some isb ->
-     xcnf unsat deduce normalise1 negate0 (if isb then pol0 else negb pol0)
-       IsBool e1
+     xcnf unsat deduce normalise1 negate0 (if isb then pol0 else negb pol0) IsBool e1
    | None ->
-     mk_iff unsat deduce (fun x x0 x1 ->
-       xcnf unsat deduce normalise1 negate0 x x0 x1) IsBool pol0 e1 e2)
+     mk_eq unsat deduce (fun x x0 x1 -> xcnf unsat deduce normalise1 negate0 x x0 x1)
+       IsBool pol0 e1 e2)
 
 (** val radd_term :
-    ('a1 -> bool) -> ('a1 -> 'a1 -> 'a1 option) -> ('a1 * 'a2) -> ('a1, 'a2)
-    clause -> (('a1, 'a2) clause, 'a2 list) sum **)
+    ('a1 -> bool) -> ('a1 -> 'a1 -> 'a1 option) -> ('a1 * 'a2) -> ('a1, 'a2) clause ->
+    (('a1, 'a2) clause, 'a2 list) sum **)
 
 let rec radd_term unsat deduce t0 = function
 | [] ->
@@ -1288,8 +1288,8 @@ let rec radd_term unsat deduce t0 = function
       | Inr l -> Inr l))
 
 (** val ror_clause :
-    ('a1 -> bool) -> ('a1 -> 'a1 -> 'a1 option) -> ('a1 * 'a2) list -> ('a1,
-    'a2) clause -> (('a1, 'a2) clause, 'a2 list) sum **)
+    ('a1 -> bool) -> ('a1 -> 'a1 -> 'a1 option) -> ('a1 * 'a2) list -> ('a1, 'a2)
+    clause -> (('a1, 'a2) clause, 'a2 list) sum **)
 
 let rec ror_clause unsat deduce cl1 cl2 =
   match cl1 with
@@ -1300,8 +1300,8 @@ let rec ror_clause unsat deduce cl1 cl2 =
      | Inr l -> Inr l)
 
 (** val xror_clause_cnf :
-    ('a1 -> bool) -> ('a1 -> 'a1 -> 'a1 option) -> ('a1 * 'a2) list -> ('a1,
-    'a2) clause list -> ('a1, 'a2) clause list * 'a2 list **)
+    ('a1 -> bool) -> ('a1 -> 'a1 -> 'a1 option) -> ('a1 * 'a2) list -> ('a1, 'a2)
+    clause list -> ('a1, 'a2) clause list * 'a2 list **)
 
 let xror_clause_cnf unsat deduce t0 f =
   fold_left (fun pat e ->
@@ -1311,8 +1311,8 @@ let xror_clause_cnf unsat deduce t0 f =
      | Inr l -> acc,(rev_append tg l))) f ([],[])
 
 (** val ror_clause_cnf :
-    ('a1 -> bool) -> ('a1 -> 'a1 -> 'a1 option) -> ('a1 * 'a2) list -> ('a1,
-    'a2) clause list -> ('a1, 'a2) clause list * 'a2 list **)
+    ('a1 -> bool) -> ('a1 -> 'a1 -> 'a1 option) -> ('a1 * 'a2) list -> ('a1, 'a2)
+    clause list -> ('a1, 'a2) clause list * 'a2 list **)
 
 let ror_clause_cnf unsat deduce t0 f =
   match t0 with
@@ -1320,8 +1320,8 @@ let ror_clause_cnf unsat deduce t0 f =
   | _::_ -> xror_clause_cnf unsat deduce t0 f
 
 (** val ror_cnf :
-    ('a1 -> bool) -> ('a1 -> 'a1 -> 'a1 option) -> ('a1, 'a2) clause list ->
-    ('a1, 'a2) clause list -> ('a1, 'a2) cnf * 'a2 list **)
+    ('a1 -> bool) -> ('a1 -> 'a1 -> 'a1 option) -> ('a1, 'a2) clause list -> ('a1,
+    'a2) clause list -> ('a1, 'a2) cnf * 'a2 list **)
 
 let rec ror_cnf unsat deduce f f' =
   match f with
@@ -1332,8 +1332,8 @@ let rec ror_cnf unsat deduce f f' =
     (rev_append rst_f' e_f'),(rev_append t0 t')
 
 (** val ror_cnf_opt :
-    ('a1 -> bool) -> ('a1 -> 'a1 -> 'a1 option) -> ('a1, 'a2) cnf -> ('a1,
-    'a2) cnf -> ('a1, 'a2) cnf * 'a2 list **)
+    ('a1 -> bool) -> ('a1 -> 'a1 -> 'a1 option) -> ('a1, 'a2) cnf -> ('a1, 'a2) cnf ->
+    ('a1, 'a2) cnf * 'a2 list **)
 
 let ror_cnf_opt unsat deduce f1 f2 =
   if is_cnf_tt f1
@@ -1347,39 +1347,39 @@ let ror_cnf_opt unsat deduce f1 f2 =
 let ratom c a =
   if if is_cnf_ff c then true else is_cnf_tt c then c,(a::[]) else c,[]
 
+(** val rxcnf_and_cnf :
+    ('a1 -> bool) -> ('a1 -> 'a1 -> 'a1 option) -> bool -> (('a1, 'a2) cnf * 'a2 list)
+    -> (('a1, 'a2) cnf * 'a2 list) -> ('a1, 'a2) cnf * 'a2 list **)
+
+let rxcnf_and_cnf unsat deduce polarity c1 c2 =
+  let e1,t1 = c1 in
+  let e2,t2 = c2 in
+  if polarity
+  then (and_cnf_opt e1 e2),(rev_append t1 t2)
+  else let f',t' = ror_cnf_opt unsat deduce e1 e2 in
+       f',(rev_append t1 (rev_append t2 t'))
+
 (** val rxcnf_and :
-    ('a2 -> bool) -> ('a2 -> 'a2 -> 'a2 option) -> (bool -> kind -> ('a1,
-    'a3, 'a4, 'a5) tFormula -> ('a2, 'a3) cnf * 'a3 list) -> bool -> kind ->
-    ('a1, 'a3, 'a4, 'a5) tFormula -> ('a1, 'a3, 'a4, 'a5) tFormula -> ('a2,
-    'a3) cnf * 'a3 list **)
+    ('a2 -> bool) -> ('a2 -> 'a2 -> 'a2 option) -> (bool -> kind -> ('a1, 'a3, 'a4,
+    'a5) tFormula -> ('a2, 'a3) cnf * 'a3 list) -> bool -> kind -> ('a1, 'a3, 'a4,
+    'a5) tFormula -> ('a1, 'a3, 'a4, 'a5) tFormula -> ('a2, 'a3) cnf * 'a3 list **)
 
 let rxcnf_and unsat deduce rXCNF polarity k e1 e2 =
-  let e3,t1 = rXCNF polarity k e1 in
-  let e4,t2 = rXCNF polarity k e2 in
-  if polarity
-  then (and_cnf_opt e3 e4),(rev_append t1 t2)
-  else let f',t' = ror_cnf_opt unsat deduce e3 e4 in
-       f',(rev_append t1 (rev_append t2 t'))
+  rxcnf_and_cnf unsat deduce polarity (rXCNF polarity k e1) (rXCNF polarity k e2)
 
 (** val rxcnf_or :
-    ('a2 -> bool) -> ('a2 -> 'a2 -> 'a2 option) -> (bool -> kind -> ('a1,
-    'a3, 'a4, 'a5) tFormula -> ('a2, 'a3) cnf * 'a3 list) -> bool -> kind ->
-    ('a1, 'a3, 'a4, 'a5) tFormula -> ('a1, 'a3, 'a4, 'a5) tFormula -> ('a2,
-    'a3) cnf * 'a3 list **)
+    ('a2 -> bool) -> ('a2 -> 'a2 -> 'a2 option) -> (bool -> kind -> ('a1, 'a3, 'a4,
+    'a5) tFormula -> ('a2, 'a3) cnf * 'a3 list) -> bool -> kind -> ('a1, 'a3, 'a4,
+    'a5) tFormula -> ('a1, 'a3, 'a4, 'a5) tFormula -> ('a2, 'a3) cnf * 'a3 list **)
 
 let rxcnf_or unsat deduce rXCNF polarity k e1 e2 =
-  let e3,t1 = rXCNF polarity k e1 in
-  let e4,t2 = rXCNF polarity k e2 in
-  if polarity
-  then let f',t' = ror_cnf_opt unsat deduce e3 e4 in
-       f',(rev_append t1 (rev_append t2 t'))
-  else (and_cnf_opt e3 e4),(rev_append t1 t2)
+  rxcnf_and_cnf unsat deduce (negb polarity) (rXCNF polarity k e1)
+    (rXCNF polarity k e2)
 
 (** val rxcnf_impl :
-    ('a2 -> bool) -> ('a2 -> 'a2 -> 'a2 option) -> (bool -> kind -> ('a1,
-    'a3, 'a4, 'a5) tFormula -> ('a2, 'a3) cnf * 'a3 list) -> bool -> kind ->
-    ('a1, 'a3, 'a4, 'a5) tFormula -> ('a1, 'a3, 'a4, 'a5) tFormula -> ('a2,
-    'a3) cnf * 'a3 list **)
+    ('a2 -> bool) -> ('a2 -> 'a2 -> 'a2 option) -> (bool -> kind -> ('a1, 'a3, 'a4,
+    'a5) tFormula -> ('a2, 'a3) cnf * 'a3 list) -> bool -> kind -> ('a1, 'a3, 'a4,
+    'a5) tFormula -> ('a1, 'a3, 'a4, 'a5) tFormula -> ('a2, 'a3) cnf * 'a3 list **)
 
 let rxcnf_impl unsat deduce rXCNF polarity k e1 e2 =
   let e3,t1 = rXCNF (negb polarity) k e1 in
@@ -1389,56 +1389,53 @@ let rxcnf_impl unsat deduce rXCNF polarity k e1 e2 =
        else let e4,t2 = rXCNF polarity k e2 in
             let f',t' = ror_cnf_opt unsat deduce e3 e4 in
             f',(rev_append t1 (rev_append t2 t'))
-  else let e4,t2 = rXCNF polarity k e2 in
-       (and_cnf_opt e3 e4),(rev_append t1 t2)
+  else let e4,t2 = rXCNF polarity k e2 in (and_cnf_opt e3 e4),(rev_append t1 t2)
 
-(** val rxcnf_iff :
-    ('a2 -> bool) -> ('a2 -> 'a2 -> 'a2 option) -> (bool -> kind -> ('a1,
-    'a3, 'a4, 'a5) tFormula -> ('a2, 'a3) cnf * 'a3 list) -> bool -> kind ->
-    ('a1, 'a3, 'a4, 'a5) tFormula -> ('a1, 'a3, 'a4, 'a5) tFormula -> ('a2,
-    'a3) cnf * 'a3 list **)
+(** val rxcnf_eq :
+    ('a2 -> bool) -> ('a2 -> 'a2 -> 'a2 option) -> (bool -> kind -> ('a1, 'a3, 'a4,
+    'a5) tFormula -> ('a2, 'a3) cnf * 'a3 list) -> bool -> kind -> ('a1, 'a3, 'a4,
+    'a5) tFormula -> ('a1, 'a3, 'a4, 'a5) tFormula -> ('a2, 'a3) cnf * 'a3 list **)
 
-let rxcnf_iff unsat deduce rXCNF polarity k e1 e2 =
+let rxcnf_eq unsat deduce rXCNF polarity k e1 e2 =
   let c1,t1 = rXCNF (negb polarity) k e1 in
   let c2,t2 = rXCNF false k e2 in
   let c3,t3 = rXCNF polarity k e1 in
   let c4,t4 = rXCNF true k e2 in
-  let f',t' = ror_cnf_opt unsat deduce (and_cnf_opt c1 c2) (and_cnf_opt c3 c4)
-  in
+  let f',t' = ror_cnf_opt unsat deduce (and_cnf_opt c1 c2) (and_cnf_opt c3 c4) in
   f',(rev_append t1 (rev_append t2 (rev_append t3 (rev_append t4 t'))))
 
 (** val rxcnf :
-    ('a2 -> bool) -> ('a2 -> 'a2 -> 'a2 option) -> ('a1 -> 'a3 -> ('a2, 'a3)
-    cnf) -> ('a1 -> 'a3 -> ('a2, 'a3) cnf) -> bool -> kind -> ('a1, 'a3, 'a4,
+    ('a2 -> bool) -> ('a2 -> 'a2 -> 'a2 option) -> (kind -> 'a1 -> 'a3 -> ('a2, 'a3)
+    cnf) -> (kind -> 'a1 -> 'a3 -> ('a2, 'a3) cnf) -> bool -> kind -> ('a1, 'a3, 'a4,
     'a5) tFormula -> ('a2, 'a3) cnf * 'a3 list **)
 
-let rec rxcnf unsat deduce normalise1 negate0 polarity _ = function
+let rec rxcnf unsat deduce normalise1 negate0 polarity k = function
 | TT _ -> if polarity then cnf_tt,[] else cnf_ff,[]
 | FF _ -> if polarity then cnf_ff,[] else cnf_tt,[]
 | X (_, _) -> cnf_ff,[]
-| A (_, x, t0) ->
-  ratom (if polarity then normalise1 x t0 else negate0 x t0) t0
+| A (_, x, t0) -> ratom (if polarity then normalise1 k x t0 else negate0 k x t0) t0
 | AND (k0, e1, e2) ->
   rxcnf_and unsat deduce (fun x x0 x1 ->
     rxcnf unsat deduce normalise1 negate0 x x0 x1) polarity k0 e1 e2
 | OR (k0, e1, e2) ->
-  rxcnf_or unsat deduce (fun x x0 x1 ->
-    rxcnf unsat deduce normalise1 negate0 x x0 x1) polarity k0 e1 e2
+  rxcnf_or unsat deduce (fun x x0 x1 -> rxcnf unsat deduce normalise1 negate0 x x0 x1)
+    polarity k0 e1 e2
 | NOT (k0, e) -> rxcnf unsat deduce normalise1 negate0 (negb polarity) k0 e
 | IMPL (k0, e1, _, e2) ->
   rxcnf_impl unsat deduce (fun x x0 x1 ->
     rxcnf unsat deduce normalise1 negate0 x x0 x1) polarity k0 e1 e2
 | IFF (k0, e1, e2) ->
-  rxcnf_iff unsat deduce (fun x x0 x1 ->
-    rxcnf unsat deduce normalise1 negate0 x x0 x1) polarity k0 e1 e2
+  rxcnf_and_cnf unsat deduce polarity
+    (rxcnf_impl unsat deduce (fun x x0 x1 ->
+      rxcnf unsat deduce normalise1 negate0 x x0 x1) polarity k0 e1 e2)
+    (rxcnf_impl unsat deduce (fun x x0 x1 ->
+      rxcnf unsat deduce normalise1 negate0 x x0 x1) polarity k0 e2 e1)
 | EQ (e1, e2) ->
-  rxcnf_iff unsat deduce (fun x x0 x1 ->
-    rxcnf unsat deduce normalise1 negate0 x x0 x1) polarity IsBool e1 e2
+  rxcnf_eq unsat deduce (fun x x0 x1 -> rxcnf unsat deduce normalise1 negate0 x x0 x1)
+    polarity IsBool e1 e2
 
-type ('term, 'annot, 'tX) to_constrT = { mkTT : (kind -> 'tX);
-                                         mkFF : (kind -> 'tX);
-                                         mkA : (kind -> 'term -> 'annot ->
-                                               'tX);
+type ('term, 'annot, 'tX) to_constrT = { mkTT : (kind -> 'tX); mkFF : (kind -> 'tX);
+                                         mkA : (kind -> 'term -> 'annot -> 'tX);
                                          mkAND : (kind -> 'tX -> 'tX -> 'tX);
                                          mkOR : (kind -> 'tX -> 'tX -> 'tX);
                                          mkIMPL : (kind -> 'tX -> 'tX -> 'tX);
@@ -1473,10 +1470,9 @@ let is_X _ = function
 | _ -> None
 
 (** val abs_and :
-    ('a1, 'a2, 'a3) to_constrT -> kind -> ('a1, 'a2, 'a3, 'a4) tFormula ->
-    ('a1, 'a2, 'a3, 'a4) tFormula -> (kind -> ('a1, 'a2, 'a3, 'a4) tFormula
-    -> ('a1, 'a2, 'a3, 'a4) tFormula -> ('a1, 'a2, 'a3, 'a4) tFormula) ->
-    ('a1, 'a3, 'a2, 'a4) gFormula **)
+    ('a1, 'a2, 'a3) to_constrT -> kind -> ('a1, 'a2, 'a3, 'a4) tFormula -> ('a1, 'a2,
+    'a3, 'a4) tFormula -> (kind -> ('a1, 'a2, 'a3, 'a4) tFormula -> ('a1, 'a2, 'a3,
+    'a4) tFormula -> ('a1, 'a2, 'a3, 'a4) tFormula) -> ('a1, 'a3, 'a2, 'a4) gFormula **)
 
 let abs_and to_constr k f1 f2 c =
   match is_X k f1 with
@@ -1487,10 +1483,9 @@ let abs_and to_constr k f1 f2 c =
      | None -> c k f1 f2)
 
 (** val abs_or :
-    ('a1, 'a2, 'a3) to_constrT -> kind -> ('a1, 'a2, 'a3, 'a4) tFormula ->
-    ('a1, 'a2, 'a3, 'a4) tFormula -> (kind -> ('a1, 'a2, 'a3, 'a4) tFormula
-    -> ('a1, 'a2, 'a3, 'a4) tFormula -> ('a1, 'a2, 'a3, 'a4) tFormula) ->
-    ('a1, 'a3, 'a2, 'a4) gFormula **)
+    ('a1, 'a2, 'a3) to_constrT -> kind -> ('a1, 'a2, 'a3, 'a4) tFormula -> ('a1, 'a2,
+    'a3, 'a4) tFormula -> (kind -> ('a1, 'a2, 'a3, 'a4) tFormula -> ('a1, 'a2, 'a3,
+    'a4) tFormula -> ('a1, 'a2, 'a3, 'a4) tFormula) -> ('a1, 'a3, 'a2, 'a4) gFormula **)
 
 let abs_or to_constr k f1 f2 c =
   match is_X k f1 with
@@ -1501,9 +1496,9 @@ let abs_or to_constr k f1 f2 c =
   | None -> c k f1 f2
 
 (** val abs_not :
-    ('a1, 'a2, 'a3) to_constrT -> kind -> ('a1, 'a2, 'a3, 'a4) tFormula ->
-    (kind -> ('a1, 'a2, 'a3, 'a4) tFormula -> ('a1, 'a2, 'a3, 'a4) tFormula)
-    -> ('a1, 'a3, 'a2, 'a4) gFormula **)
+    ('a1, 'a2, 'a3) to_constrT -> kind -> ('a1, 'a2, 'a3, 'a4) tFormula -> (kind ->
+    ('a1, 'a2, 'a3, 'a4) tFormula -> ('a1, 'a2, 'a3, 'a4) tFormula) -> ('a1, 'a3, 'a2,
+    'a4) gFormula **)
 
 let abs_not to_constr k f1 c =
   match is_X k f1 with
@@ -1511,73 +1506,63 @@ let abs_not to_constr k f1 c =
   | None -> c k f1
 
 (** val mk_arrow :
-    'a4 option -> kind -> ('a1, 'a2, 'a3, 'a4) tFormula -> ('a1, 'a2, 'a3,
-    'a4) tFormula -> ('a1, 'a2, 'a3, 'a4) tFormula **)
+    'a4 option -> kind -> ('a1, 'a2, 'a3, 'a4) tFormula -> ('a1, 'a2, 'a3, 'a4)
+    tFormula -> ('a1, 'a2, 'a3, 'a4) tFormula **)
 
 let mk_arrow o k f1 f2 =
   match o with
-  | Some _ ->
-    (match is_X k f1 with
-     | Some _ -> f2
-     | None -> IMPL (k, f1, o, f2))
+  | Some _ -> (match is_X k f1 with
+               | Some _ -> f2
+               | None -> IMPL (k, f1, o, f2))
   | None -> IMPL (k, f1, None, f2)
 
 (** val abst_simpl :
-    ('a1, 'a2, 'a3) to_constrT -> ('a2 -> bool) -> kind -> ('a1, 'a2, 'a3,
-    'a4) tFormula -> ('a1, 'a2, 'a3, 'a4) tFormula **)
+    ('a1, 'a2, 'a3) to_constrT -> ('a2 -> bool) -> kind -> ('a1, 'a2, 'a3, 'a4)
+    tFormula -> ('a1, 'a2, 'a3, 'a4) tFormula **)
 
 let rec abst_simpl to_constr needA _ = function
-| A (k, x, t0) ->
-  if needA t0 then A (k, x, t0) else X (k, (to_constr.mkA k x t0))
+| A (k, x, t0) -> if needA t0 then A (k, x, t0) else X (k, (to_constr.mkA k x t0))
 | AND (k0, f1, f2) ->
-  AND (k0, (abst_simpl to_constr needA k0 f1),
-    (abst_simpl to_constr needA k0 f2))
+  AND (k0, (abst_simpl to_constr needA k0 f1), (abst_simpl to_constr needA k0 f2))
 | OR (k0, f1, f2) ->
-  OR (k0, (abst_simpl to_constr needA k0 f1),
-    (abst_simpl to_constr needA k0 f2))
+  OR (k0, (abst_simpl to_constr needA k0 f1), (abst_simpl to_constr needA k0 f2))
 | NOT (k0, f0) -> NOT (k0, (abst_simpl to_constr needA k0 f0))
 | IMPL (k0, f1, o, f2) ->
-  IMPL (k0, (abst_simpl to_constr needA k0 f1), o,
-    (abst_simpl to_constr needA k0 f2))
+  IMPL (k0, (abst_simpl to_constr needA k0 f1), o, (abst_simpl to_constr needA k0 f2))
 | IFF (k0, f1, f2) ->
-  IFF (k0, (abst_simpl to_constr needA k0 f1),
-    (abst_simpl to_constr needA k0 f2))
+  IFF (k0, (abst_simpl to_constr needA k0 f1), (abst_simpl to_constr needA k0 f2))
 | EQ (f1, f2) ->
-  EQ ((abst_simpl to_constr needA IsBool f1),
-    (abst_simpl to_constr needA IsBool f2))
+  EQ ((abst_simpl to_constr needA IsBool f1), (abst_simpl to_constr needA IsBool f2))
 | x -> x
 
 (** val abst_and :
-    ('a1, 'a2, 'a3) to_constrT -> (bool -> kind -> ('a1, 'a2, 'a3, 'a4)
-    tFormula -> ('a1, 'a2, 'a3, 'a4) tFormula) -> bool -> kind -> ('a1, 'a2,
-    'a3, 'a4) tFormula -> ('a1, 'a2, 'a3, 'a4) tFormula -> ('a1, 'a2, 'a3,
-    'a4) tFormula **)
+    ('a1, 'a2, 'a3) to_constrT -> (bool -> kind -> ('a1, 'a2, 'a3, 'a4) tFormula ->
+    ('a1, 'a2, 'a3, 'a4) tFormula) -> bool -> kind -> ('a1, 'a2, 'a3, 'a4) tFormula ->
+    ('a1, 'a2, 'a3, 'a4) tFormula -> ('a1, 'a2, 'a3, 'a4) tFormula **)
 
 let abst_and to_constr rEC pol0 k f1 f2 =
   if pol0
-  then abs_and to_constr k (rEC pol0 k f1) (rEC pol0 k f2) (fun x x0 x1 ->
-         AND (x, x0, x1))
-  else abs_or to_constr k (rEC pol0 k f1) (rEC pol0 k f2) (fun x x0 x1 -> AND
-         (x, x0, x1))
+  then abs_and to_constr k (rEC pol0 k f1) (rEC pol0 k f2) (fun x x0 x1 -> AND (x, x0,
+         x1))
+  else abs_or to_constr k (rEC pol0 k f1) (rEC pol0 k f2) (fun x x0 x1 -> AND (x, x0,
+         x1))
 
 (** val abst_or :
-    ('a1, 'a2, 'a3) to_constrT -> (bool -> kind -> ('a1, 'a2, 'a3, 'a4)
-    tFormula -> ('a1, 'a2, 'a3, 'a4) tFormula) -> bool -> kind -> ('a1, 'a2,
-    'a3, 'a4) tFormula -> ('a1, 'a2, 'a3, 'a4) tFormula -> ('a1, 'a2, 'a3,
-    'a4) tFormula **)
+    ('a1, 'a2, 'a3) to_constrT -> (bool -> kind -> ('a1, 'a2, 'a3, 'a4) tFormula ->
+    ('a1, 'a2, 'a3, 'a4) tFormula) -> bool -> kind -> ('a1, 'a2, 'a3, 'a4) tFormula ->
+    ('a1, 'a2, 'a3, 'a4) tFormula -> ('a1, 'a2, 'a3, 'a4) tFormula **)
 
 let abst_or to_constr rEC pol0 k f1 f2 =
   if pol0
-  then abs_or to_constr k (rEC pol0 k f1) (rEC pol0 k f2) (fun x x0 x1 -> OR
-         (x, x0, x1))
-  else abs_and to_constr k (rEC pol0 k f1) (rEC pol0 k f2) (fun x x0 x1 -> OR
-         (x, x0, x1))
+  then abs_or to_constr k (rEC pol0 k f1) (rEC pol0 k f2) (fun x x0 x1 -> OR (x, x0,
+         x1))
+  else abs_and to_constr k (rEC pol0 k f1) (rEC pol0 k f2) (fun x x0 x1 -> OR (x, x0,
+         x1))
 
 (** val abst_impl :
-    ('a1, 'a2, 'a3) to_constrT -> (bool -> kind -> ('a1, 'a2, 'a3, 'a4)
-    tFormula -> ('a1, 'a2, 'a3, 'a4) tFormula) -> bool -> 'a4 option -> kind
-    -> ('a1, 'a2, 'a3, 'a4) tFormula -> ('a1, 'a2, 'a3, 'a4) tFormula ->
-    ('a1, 'a2, 'a3, 'a4) tFormula **)
+    ('a1, 'a2, 'a3) to_constrT -> (bool -> kind -> ('a1, 'a2, 'a3, 'a4) tFormula ->
+    ('a1, 'a2, 'a3, 'a4) tFormula) -> bool -> 'a4 option -> kind -> ('a1, 'a2, 'a3,
+    'a4) tFormula -> ('a1, 'a2, 'a3, 'a4) tFormula -> ('a1, 'a2, 'a3, 'a4) tFormula **)
 
 let abst_impl to_constr rEC pol0 o k f1 f2 =
   if pol0
@@ -1585,8 +1570,7 @@ let abst_impl to_constr rEC pol0 o k f1 f2 =
   else abs_and to_constr k (rEC (negb pol0) k f1) (rEC pol0 k f2) (mk_arrow o)
 
 (** val or_is_X :
-    kind -> ('a1, 'a2, 'a3, 'a4) tFormula -> ('a1, 'a2, 'a3, 'a4) tFormula ->
-    bool **)
+    kind -> ('a1, 'a2, 'a3, 'a4) tFormula -> ('a1, 'a2, 'a3, 'a4) tFormula -> bool **)
 
 let or_is_X k f1 f2 =
   match is_X k f1 with
@@ -1596,62 +1580,61 @@ let or_is_X k f1 f2 =
              | None -> false)
 
 (** val abs_iff :
-    ('a1, 'a2, 'a3) to_constrT -> kind -> ('a1, 'a2, 'a3, 'a4) tFormula ->
-    ('a1, 'a2, 'a3, 'a4) tFormula -> ('a1, 'a2, 'a3, 'a4) tFormula -> ('a1,
-    'a2, 'a3, 'a4) tFormula -> kind -> ('a1, 'a2, 'a3, 'a4) tFormula -> ('a1,
-    'a2, 'a3, 'a4) tFormula **)
+    kind -> ('a1, 'a2, 'a3, 'a4) tFormula -> ('a1, 'a2, 'a3, 'a4) tFormula -> ('a1,
+    'a2, 'a3, 'a4) tFormula -> ('a1, 'a2, 'a3, 'a4) tFormula -> ('a1, 'a2, 'a3, 'a4)
+    tFormula -> ('a1, 'a2, 'a3, 'a4) tFormula **)
 
-let abs_iff to_constr k nf1 ff2 f1 tf2 r def =
+let abs_iff _ _ _ _ _ def =
+  def
+
+(** val abst_iff :
+    ('a1, 'a2, 'a3) to_constrT -> ('a2 -> bool) -> (bool -> kind -> ('a1, 'a2, 'a3,
+    'a4) tFormula -> ('a1, 'a2, 'a3, 'a4) tFormula) -> bool -> kind -> ('a1, 'a2, 'a3,
+    'a4) tFormula -> ('a1, 'a2, 'a3, 'a4) tFormula -> ('a1, 'a2, 'a3, 'a4) tFormula **)
+
+let abst_iff to_constr needA rEC pol0 k f1 f2 =
+  abs_iff k (rEC (negb pol0) k f1) (rEC false k f2) (rEC pol0 k f1) (rEC true k f2)
+    (IFF (k, (abst_simpl to_constr needA k f1), (abst_simpl to_constr needA k f2)))
+
+(** val abs_eq :
+    ('a1, 'a2, 'a3) to_constrT -> kind -> ('a1, 'a2, 'a3, 'a4) tFormula -> ('a1, 'a2,
+    'a3, 'a4) tFormula -> ('a1, 'a2, 'a3, 'a4) tFormula -> ('a1, 'a2, 'a3, 'a4)
+    tFormula -> kind -> ('a1, 'a2, 'a3, 'a4) tFormula -> ('a1, 'a2, 'a3, 'a4) tFormula **)
+
+let abs_eq to_constr k nf1 ff2 f1 tf2 r def =
   if (&&) (or_is_X k nf1 ff2) (or_is_X k f1 tf2)
   then X (r, (aformula to_constr r def))
   else def
 
-(** val abst_iff :
-    ('a1, 'a2, 'a3) to_constrT -> ('a2 -> bool) -> (bool -> kind -> ('a1,
-    'a2, 'a3, 'a4) tFormula -> ('a1, 'a2, 'a3, 'a4) tFormula) -> bool -> kind
-    -> ('a1, 'a2, 'a3, 'a4) tFormula -> ('a1, 'a2, 'a3, 'a4) tFormula ->
-    ('a1, 'a2, 'a3, 'a4) tFormula **)
-
-let abst_iff to_constr needA rEC pol0 k f1 f2 =
-  abs_iff to_constr k (rEC (negb pol0) k f1) (rEC false k f2) (rEC pol0 k f1)
-    (rEC true k f2) k (IFF (k, (abst_simpl to_constr needA k f1),
-    (abst_simpl to_constr needA k f2)))
-
 (** val abst_eq :
-    ('a1, 'a2, 'a3) to_constrT -> ('a2 -> bool) -> (bool -> kind -> ('a1,
-    'a2, 'a3, 'a4) tFormula -> ('a1, 'a2, 'a3, 'a4) tFormula) -> bool ->
-    ('a1, 'a2, 'a3, 'a4) tFormula -> ('a1, 'a2, 'a3, 'a4) tFormula -> ('a1,
-    'a2, 'a3, 'a4) tFormula **)
+    ('a1, 'a2, 'a3) to_constrT -> ('a2 -> bool) -> (bool -> kind -> ('a1, 'a2, 'a3,
+    'a4) tFormula -> ('a1, 'a2, 'a3, 'a4) tFormula) -> bool -> ('a1, 'a2, 'a3, 'a4)
+    tFormula -> ('a1, 'a2, 'a3, 'a4) tFormula -> ('a1, 'a2, 'a3, 'a4) tFormula **)
 
 let abst_eq to_constr needA rEC pol0 f1 f2 =
-  abs_iff to_constr IsBool (rEC (negb pol0) IsBool f1) (rEC false IsBool f2)
+  abs_eq to_constr IsBool (rEC (negb pol0) IsBool f1) (rEC false IsBool f2)
     (rEC pol0 IsBool f1) (rEC true IsBool f2) IsProp (EQ
-    ((abst_simpl to_constr needA IsBool f1),
-    (abst_simpl to_constr needA IsBool f2)))
+    ((abst_simpl to_constr needA IsBool f1), (abst_simpl to_constr needA IsBool f2)))
 
 (** val abst_form :
-    ('a1, 'a2, 'a3) to_constrT -> ('a2 -> bool) -> bool -> kind -> ('a1, 'a2,
-    'a3, 'a4) tFormula -> ('a1, 'a2, 'a3, 'a4) tFormula **)
+    ('a1, 'a2, 'a3) to_constrT -> ('a2 -> bool) -> bool -> kind -> ('a1, 'a2, 'a3,
+    'a4) tFormula -> ('a1, 'a2, 'a3, 'a4) tFormula **)
 
 let rec abst_form to_constr needA pol0 _ = function
 | TT k -> if pol0 then TT k else X (k, (to_constr.mkTT k))
 | FF k -> if pol0 then X (k, (to_constr.mkFF k)) else FF k
 | X (k, p) -> X (k, p)
-| A (k, x, t0) ->
-  if needA t0 then A (k, x, t0) else X (k, (to_constr.mkA k x t0))
-| AND (k0, f1, f2) ->
-  abst_and to_constr (abst_form to_constr needA) pol0 k0 f1 f2
-| OR (k0, f1, f2) ->
-  abst_or to_constr (abst_form to_constr needA) pol0 k0 f1 f2
+| A (k, x, t0) -> if needA t0 then A (k, x, t0) else X (k, (to_constr.mkA k x t0))
+| AND (k0, f1, f2) -> abst_and to_constr (abst_form to_constr needA) pol0 k0 f1 f2
+| OR (k0, f1, f2) -> abst_or to_constr (abst_form to_constr needA) pol0 k0 f1 f2
 | NOT (k0, f0) ->
-  abs_not to_constr k0 (abst_form to_constr needA (negb pol0) k0 f0)
-    (fun x x0 -> NOT (x, x0))
+  abs_not to_constr k0 (abst_form to_constr needA (negb pol0) k0 f0) (fun x x0 -> NOT
+    (x, x0))
 | IMPL (k0, f1, o, f2) ->
   abst_impl to_constr (abst_form to_constr needA) pol0 o k0 f1 f2
 | IFF (k0, f1, f2) ->
   abst_iff to_constr needA (abst_form to_constr needA) pol0 k0 f1 f2
-| EQ (f1, f2) ->
-  abst_eq to_constr needA (abst_form to_constr needA) pol0 f1 f2
+| EQ (f1, f2) -> abst_eq to_constr needA (abst_form to_constr needA) pol0 f1 f2
 
 (** val cnf_checker :
     (('a1 * 'a2) list -> 'a3 -> bool) -> ('a1, 'a2) cnf -> 'a3 list -> bool **)
@@ -1665,8 +1648,8 @@ let rec cnf_checker checker f l =
      | c::l0 -> if checker e c then cnf_checker checker f0 l0 else false)
 
 (** val tauto_checker :
-    ('a2 -> bool) -> ('a2 -> 'a2 -> 'a2 option) -> ('a1 -> 'a3 -> ('a2, 'a3)
-    cnf) -> ('a1 -> 'a3 -> ('a2, 'a3) cnf) -> (('a2 * 'a3) list -> 'a4 ->
+    ('a2 -> bool) -> ('a2 -> 'a2 -> 'a2 option) -> (kind -> 'a1 -> 'a3 -> ('a2, 'a3)
+    cnf) -> (kind -> 'a1 -> 'a3 -> ('a2, 'a3) cnf) -> (('a2 * 'a3) list -> 'a4 ->
     bool) -> ('a1, rtyp, 'a3, unit0) gFormula -> 'a4 list -> bool **)
 
 let tauto_checker unsat deduce normalise1 negate0 checker f w =
@@ -1677,8 +1660,7 @@ let tauto_checker unsat deduce normalise1 negate0 checker f w =
 let cneqb ceqb x y =
   negb (ceqb x y)
 
-(** val cltb :
-    ('a1 -> 'a1 -> bool) -> ('a1 -> 'a1 -> bool) -> 'a1 -> 'a1 -> bool **)
+(** val cltb : ('a1 -> 'a1 -> bool) -> ('a1 -> 'a1 -> bool) -> 'a1 -> 'a1 -> bool **)
 
 let cltb ceqb cleb x y =
   (&&) (cleb x y) (cneqb ceqb x y)
@@ -1755,8 +1737,8 @@ let map_option2 f o o' =
   | None -> None
 
 (** val pexpr_times_nformula :
-    'a1 -> 'a1 -> ('a1 -> 'a1 -> 'a1) -> ('a1 -> 'a1 -> 'a1) -> ('a1 -> 'a1
-    -> bool) -> 'a1 polC -> 'a1 nFormula -> 'a1 nFormula option **)
+    'a1 -> 'a1 -> ('a1 -> 'a1 -> 'a1) -> ('a1 -> 'a1 -> 'a1) -> ('a1 -> 'a1 -> bool)
+    -> 'a1 polC -> 'a1 nFormula -> 'a1 nFormula option **)
 
 let pexpr_times_nformula cO cI cplus ctimes ceqb e = function
 | ef,o ->
@@ -1765,18 +1747,17 @@ let pexpr_times_nformula cO cI cplus ctimes ceqb e = function
    | _ -> None)
 
 (** val nformula_times_nformula :
-    'a1 -> 'a1 -> ('a1 -> 'a1 -> 'a1) -> ('a1 -> 'a1 -> 'a1) -> ('a1 -> 'a1
-    -> bool) -> 'a1 nFormula -> 'a1 nFormula -> 'a1 nFormula option **)
+    'a1 -> 'a1 -> ('a1 -> 'a1 -> 'a1) -> ('a1 -> 'a1 -> 'a1) -> ('a1 -> 'a1 -> bool)
+    -> 'a1 nFormula -> 'a1 nFormula -> 'a1 nFormula option **)
 
 let nformula_times_nformula cO cI cplus ctimes ceqb f1 f2 =
   let e1,o1 = f1 in
   let e2,o2 = f2 in
-  map_option (fun x -> Some ((pmul cO cI cplus ctimes ceqb e1 e2),x))
-    (opMult o1 o2)
+  map_option (fun x -> Some ((pmul cO cI cplus ctimes ceqb e1 e2),x)) (opMult o1 o2)
 
 (** val nformula_plus_nformula :
-    'a1 -> ('a1 -> 'a1 -> 'a1) -> ('a1 -> 'a1 -> bool) -> 'a1 nFormula -> 'a1
-    nFormula -> 'a1 nFormula option **)
+    'a1 -> ('a1 -> 'a1 -> 'a1) -> ('a1 -> 'a1 -> bool) -> 'a1 nFormula -> 'a1 nFormula
+    -> 'a1 nFormula option **)
 
 let nformula_plus_nformula cO cplus ceqb f1 f2 =
   let e1,o1 = f1 in
@@ -1784,9 +1765,8 @@ let nformula_plus_nformula cO cplus ceqb f1 f2 =
   map_option (fun x -> Some ((padd cO cplus ceqb e1 e2),x)) (opAdd o1 o2)
 
 (** val eval_Psatz :
-    'a1 -> 'a1 -> ('a1 -> 'a1 -> 'a1) -> ('a1 -> 'a1 -> 'a1) -> ('a1 -> 'a1
-    -> bool) -> ('a1 -> 'a1 -> bool) -> 'a1 nFormula list -> 'a1 psatz -> 'a1
-    nFormula option **)
+    'a1 -> 'a1 -> ('a1 -> 'a1 -> 'a1) -> ('a1 -> 'a1 -> 'a1) -> ('a1 -> 'a1 -> bool)
+    -> ('a1 -> 'a1 -> bool) -> 'a1 nFormula list -> 'a1 psatz -> 'a1 nFormula option **)
 
 let rec eval_Psatz cO cI cplus ctimes ceqb cleb l = function
 | PsatzIn n0 -> Some (nth n0 l ((Pc cO),Equal))
@@ -1806,8 +1786,7 @@ let rec eval_Psatz cO cI cplus ctimes ceqb cleb l = function
 | PsatzZ -> Some ((Pc cO),Equal)
 
 (** val check_inconsistent :
-    'a1 -> ('a1 -> 'a1 -> bool) -> ('a1 -> 'a1 -> bool) -> 'a1 nFormula ->
-    bool **)
+    'a1 -> ('a1 -> 'a1 -> bool) -> ('a1 -> 'a1 -> bool) -> 'a1 nFormula -> bool **)
 
 let check_inconsistent cO ceqb cleb = function
 | e,op ->
@@ -1821,8 +1800,8 @@ let check_inconsistent cO ceqb cleb = function
    | _ -> false)
 
 (** val check_normalised_formulas :
-    'a1 -> 'a1 -> ('a1 -> 'a1 -> 'a1) -> ('a1 -> 'a1 -> 'a1) -> ('a1 -> 'a1
-    -> bool) -> ('a1 -> 'a1 -> bool) -> 'a1 nFormula list -> 'a1 psatz -> bool **)
+    'a1 -> 'a1 -> ('a1 -> 'a1 -> 'a1) -> ('a1 -> 'a1 -> 'a1) -> ('a1 -> 'a1 -> bool)
+    -> ('a1 -> 'a1 -> bool) -> 'a1 nFormula list -> 'a1 psatz -> bool **)
 
 let check_normalised_formulas cO cI cplus ctimes ceqb cleb l cm =
   match eval_Psatz cO cI cplus ctimes ceqb cleb l cm with
@@ -1840,22 +1819,21 @@ type op2 =
 type 't formula = { flhs : 't pExpr; fop : op2; frhs : 't pExpr }
 
 (** val norm :
-    'a1 -> 'a1 -> ('a1 -> 'a1 -> 'a1) -> ('a1 -> 'a1 -> 'a1) -> ('a1 -> 'a1
-    -> 'a1) -> ('a1 -> 'a1) -> ('a1 -> 'a1 -> bool) -> 'a1 pExpr -> 'a1 pol **)
+    'a1 -> 'a1 -> ('a1 -> 'a1 -> 'a1) -> ('a1 -> 'a1 -> 'a1) -> ('a1 -> 'a1 -> 'a1) ->
+    ('a1 -> 'a1) -> ('a1 -> 'a1 -> bool) -> 'a1 pExpr -> 'a1 pol **)
 
 let norm =
   norm_aux
 
 (** val psub0 :
-    'a1 -> ('a1 -> 'a1 -> 'a1) -> ('a1 -> 'a1 -> 'a1) -> ('a1 -> 'a1) -> ('a1
-    -> 'a1 -> bool) -> 'a1 pol -> 'a1 pol -> 'a1 pol **)
+    'a1 -> ('a1 -> 'a1 -> 'a1) -> ('a1 -> 'a1 -> 'a1) -> ('a1 -> 'a1) -> ('a1 -> 'a1
+    -> bool) -> 'a1 pol -> 'a1 pol -> 'a1 pol **)
 
 let psub0 =
   psub
 
 (** val padd0 :
-    'a1 -> ('a1 -> 'a1 -> 'a1) -> ('a1 -> 'a1 -> bool) -> 'a1 pol -> 'a1 pol
-    -> 'a1 pol **)
+    'a1 -> ('a1 -> 'a1 -> 'a1) -> ('a1 -> 'a1 -> bool) -> 'a1 pol -> 'a1 pol -> 'a1 pol **)
 
 let padd0 =
   padd
@@ -1866,9 +1844,8 @@ let popp0 =
   popp
 
 (** val normalise :
-    'a1 -> 'a1 -> ('a1 -> 'a1 -> 'a1) -> ('a1 -> 'a1 -> 'a1) -> ('a1 -> 'a1
-    -> 'a1) -> ('a1 -> 'a1) -> ('a1 -> 'a1 -> bool) -> 'a1 formula -> 'a1
-    nFormula **)
+    'a1 -> 'a1 -> ('a1 -> 'a1 -> 'a1) -> ('a1 -> 'a1 -> 'a1) -> ('a1 -> 'a1 -> 'a1) ->
+    ('a1 -> 'a1) -> ('a1 -> 'a1 -> bool) -> 'a1 formula -> 'a1 nFormula **)
 
 let normalise cO cI cplus ctimes cminus copp ceqb f =
   let { flhs = lhs; fop = op; frhs = rhs } = f in
@@ -1901,18 +1878,17 @@ let xnegate copp = function
    | x -> (e,x)::[])
 
 (** val cnf_of_list :
-    'a1 -> ('a1 -> 'a1 -> bool) -> ('a1 -> 'a1 -> bool) -> 'a1 nFormula list
-    -> 'a2 -> ('a1 nFormula, 'a2) cnf **)
+    'a1 -> ('a1 -> 'a1 -> bool) -> ('a1 -> 'a1 -> bool) -> 'a1 nFormula list -> 'a2 ->
+    ('a1 nFormula, 'a2) cnf **)
 
 let cnf_of_list cO ceqb cleb l tg =
   fold_right (fun x acc ->
-    if check_inconsistent cO ceqb cleb x then acc else ((x,tg)::[])::acc)
-    cnf_tt l
+    if check_inconsistent cO ceqb cleb x then acc else ((x,tg)::[])::acc) cnf_tt l
 
 (** val cnf_normalise :
-    'a1 -> 'a1 -> ('a1 -> 'a1 -> 'a1) -> ('a1 -> 'a1 -> 'a1) -> ('a1 -> 'a1
-    -> 'a1) -> ('a1 -> 'a1) -> ('a1 -> 'a1 -> bool) -> ('a1 -> 'a1 -> bool)
-    -> 'a1 formula -> 'a2 -> ('a1 nFormula, 'a2) cnf **)
+    'a1 -> 'a1 -> ('a1 -> 'a1 -> 'a1) -> ('a1 -> 'a1 -> 'a1) -> ('a1 -> 'a1 -> 'a1) ->
+    ('a1 -> 'a1) -> ('a1 -> 'a1 -> bool) -> ('a1 -> 'a1 -> bool) -> 'a1 formula -> 'a2
+    -> ('a1 nFormula, 'a2) cnf **)
 
 let cnf_normalise cO cI cplus ctimes cminus copp ceqb cleb t0 tg =
   let f = normalise cO cI cplus ctimes cminus copp ceqb t0 in
@@ -1921,9 +1897,9 @@ let cnf_normalise cO cI cplus ctimes cminus copp ceqb cleb t0 tg =
   else cnf_of_list cO ceqb cleb (xnormalise copp f) tg
 
 (** val cnf_negate :
-    'a1 -> 'a1 -> ('a1 -> 'a1 -> 'a1) -> ('a1 -> 'a1 -> 'a1) -> ('a1 -> 'a1
-    -> 'a1) -> ('a1 -> 'a1) -> ('a1 -> 'a1 -> bool) -> ('a1 -> 'a1 -> bool)
-    -> 'a1 formula -> 'a2 -> ('a1 nFormula, 'a2) cnf **)
+    'a1 -> 'a1 -> ('a1 -> 'a1 -> 'a1) -> ('a1 -> 'a1 -> 'a1) -> ('a1 -> 'a1 -> 'a1) ->
+    ('a1 -> 'a1) -> ('a1 -> 'a1 -> bool) -> ('a1 -> 'a1 -> bool) -> 'a1 formula -> 'a2
+    -> ('a1 nFormula, 'a2) cnf **)
 
 let cnf_negate cO cI cplus ctimes cminus copp ceqb cleb t0 tg =
   let f = normalise cO cI cplus ctimes cminus copp ceqb t0 in
@@ -1963,8 +1939,7 @@ let map_Formula c_of_S f =
   { flhs = (map_PExpr c_of_S l); fop = o; frhs = (map_PExpr c_of_S r) }
 
 (** val simpl_cone :
-    'a1 -> 'a1 -> ('a1 -> 'a1 -> 'a1) -> ('a1 -> 'a1 -> bool) -> 'a1 psatz ->
-    'a1 psatz **)
+    'a1 -> 'a1 -> ('a1 -> 'a1 -> 'a1) -> ('a1 -> 'a1 -> bool) -> 'a1 psatz -> 'a1 psatz **)
 
 let simpl_cone cO cI ctimes ceqb e = match e with
 | PsatzSquare t0 ->
@@ -2035,8 +2010,8 @@ let qle_bool x y =
 (** val qplus : q -> q -> q **)
 
 let qplus x y =
-  { qnum = (Z.add (Z.mul x.qnum (Zpos y.qden)) (Z.mul y.qnum (Zpos x.qden)));
-    qden = (Coq_Pos.mul x.qden y.qden) }
+  { qnum = (Z.add (Z.mul x.qnum (Zpos y.qden)) (Z.mul y.qnum (Zpos x.qden))); qden =
+    (Coq_Pos.mul x.qden y.qden) }
 
 (** val qmult : q -> q -> q **)
 
@@ -2125,8 +2100,7 @@ let rec zeval_const = function
 | PEmul (e1, e2) ->
   map_option2 (fun x y -> Some (Z.mul x y)) (zeval_const e1) (zeval_const e2)
 | PEopp e0 -> map_option (fun x -> Some (Z.opp x)) (zeval_const e0)
-| PEpow (e1, n0) ->
-  map_option (fun x -> Some (Z.pow x (Z.of_N n0))) (zeval_const e1)
+| PEpow (e1, n0) -> map_option (fun x -> Some (Z.pow x (Z.of_N n0))) (zeval_const e1)
 
 type zWitness = z psatz
 
@@ -2185,16 +2159,14 @@ let xnormalise0 = function
    | Strict -> ((psub1 (Pc Z0) e),NonStrict)::[]
    | NonStrict -> ((psub1 (Pc (Zneg XH)) e),NonStrict)::[])
 
-(** val cnf_of_list0 :
-    'a1 -> z nFormula list -> (z nFormula * 'a1) list list **)
+(** val cnf_of_list0 : 'a1 -> z nFormula list -> (z nFormula * 'a1) list list **)
 
 let cnf_of_list0 tg l =
-  fold_right (fun x acc -> if zunsat x then acc else ((x,tg)::[])::acc)
-    cnf_tt l
+  fold_right (fun x acc -> if zunsat x then acc else ((x,tg)::[])::acc) cnf_tt l
 
-(** val normalise0 : z formula -> 'a1 -> (z nFormula, 'a1) cnf **)
+(** val normalise0 : kind -> z formula -> 'a1 -> (z nFormula, 'a1) cnf **)
 
-let normalise0 t0 tg =
+let normalise0 _ t0 tg =
   let f = xnnormalise t0 in
   if zunsat f then cnf_ff else cnf_of_list0 tg (xnormalise0 f)
 
@@ -2208,15 +2180,13 @@ let xnegate0 = function
    | Strict -> ((psub1 e (Pc (Zpos XH))),NonStrict)::[]
    | x -> (e,x)::[])
 
-(** val negate : z formula -> 'a1 -> (z nFormula, 'a1) cnf **)
+(** val negate : kind -> z formula -> 'a1 -> (z nFormula, 'a1) cnf **)
 
-let negate t0 tg =
-  let f = xnnormalise t0 in
-  if zunsat f then cnf_tt else cnf_of_list0 tg (xnegate0 f)
+let negate _ t0 tg =
+  let f = xnnormalise t0 in if zunsat f then cnf_tt else cnf_of_list0 tg (xnegate0 f)
 
 (** val cnfZ :
-    kind -> (z formula, 'a1, 'a2, 'a3) tFormula -> (z nFormula, 'a1)
-    cnf * 'a1 list **)
+    kind -> (z formula, 'a1, 'a2, 'a3) tFormula -> (z nFormula, 'a1) cnf * 'a1 list **)
 
 let cnfZ k f =
   rxcnf zunsat zdeduce normalise0 negate true k f
@@ -2224,10 +2194,9 @@ let cnfZ k f =
 (** val ceiling : z -> z -> z **)
 
 let ceiling a b =
-  let q0,r = Z.div_eucl a b in
-  (match r with
-   | Z0 -> q0
-   | _ -> Z.add q0 (Zpos XH))
+  let q0,r = Z.div_eucl a b in (match r with
+                                | Z0 -> q0
+                                | _ -> Z.add q0 (Zpos XH))
 
 type zArithProof =
 | DoneProof
@@ -2247,8 +2216,7 @@ let rec zgcd_pol = function
 | Pc c -> Z0,c
 | Pinj (_, p2) -> zgcd_pol p2
 | PX (p2, _, q0) ->
-  let g1,c1 = zgcd_pol p2 in
-  let g2,c2 = zgcd_pol q0 in (zgcdM (zgcdM g1 c1) g2),c2
+  let g1,c1 = zgcd_pol p2 in let g2,c2 = zgcd_pol q0 in (zgcdM (zgcdM g1 c1) g2),c2
 
 (** val zdiv_pol : z polC -> z -> z polC **)
 
@@ -2273,8 +2241,7 @@ let genCuttingPlane = function
   (match op with
    | Equal ->
      let g,c = zgcd_pol e in
-     if (&&) (Z.gtb g Z0)
-          ((&&) (negb (zeq_bool c Z0)) (negb (zeq_bool (Z.gcd g c) g)))
+     if (&&) (Z.gtb g Z0) ((&&) (negb (zeq_bool c Z0)) (negb (zeq_bool (Z.gcd g c) g)))
      then None
      else Some ((makeCuttingPlane e),Equal)
    | NonEqual -> Some ((e,Z0),op)
@@ -2321,8 +2288,7 @@ let mk_eq_pos x y t0 =
 let rec max_var jmp = function
 | Pc _ -> jmp
 | Pinj (j, p2) -> max_var (Coq_Pos.add j jmp) p2
-| PX (p2, _, q0) ->
-  Coq_Pos.max (max_var jmp p2) (max_var (Coq_Pos.succ jmp) q0)
+| PX (p2, _, q0) -> Coq_Pos.max (max_var jmp p2) (max_var (Coq_Pos.succ jmp) q0)
 
 (** val max_var_nformulae : z nFormula list -> positive **)
 
@@ -2378,35 +2344,33 @@ let rec zChecker l = function
        let t0 = Coq_Pos.succ z0 in
        let nfx = xnnormalise (mk_eq_pos x z0 t0) in
        let posz = xnnormalise (bound_var z0) in
-       let post = xnnormalise (bound_var t0) in
-       zChecker (nfx::(posz::(post::l))) prf
+       let post = xnnormalise (bound_var t0) in zChecker (nfx::(posz::(post::l))) prf
   else false
 
 (** val zTautoChecker : z formula bFormula -> zArithProof list -> bool **)
 
 let zTautoChecker f w =
-  tauto_checker zunsat zdeduce normalise0 negate (fun cl ->
-    zChecker (map fst cl)) f w
+  tauto_checker zunsat zdeduce normalise0 negate (fun cl -> zChecker (map fst cl)) f w
 
 type qWitness = q psatz
 
 (** val qWeakChecker : q nFormula list -> q psatz -> bool **)
 
 let qWeakChecker =
-  check_normalised_formulas { qnum = Z0; qden = XH } { qnum = (Zpos XH);
-    qden = XH } qplus qmult qeq_bool qle_bool
+  check_normalised_formulas { qnum = Z0; qden = XH } { qnum = (Zpos XH); qden = XH }
+    qplus qmult qeq_bool qle_bool
 
-(** val qnormalise : q formula -> 'a1 -> (q nFormula, 'a1) cnf **)
+(** val qnormalise : kind -> q formula -> 'a1 -> (q nFormula, 'a1) cnf **)
 
-let qnormalise t0 tg =
-  cnf_normalise { qnum = Z0; qden = XH } { qnum = (Zpos XH); qden = XH }
-    qplus qmult qminus qopp qeq_bool qle_bool t0 tg
+let qnormalise _ =
+  cnf_normalise { qnum = Z0; qden = XH } { qnum = (Zpos XH); qden = XH } qplus qmult
+    qminus qopp qeq_bool qle_bool
 
-(** val qnegate : q formula -> 'a1 -> (q nFormula, 'a1) cnf **)
+(** val qnegate : kind -> q formula -> 'a1 -> (q nFormula, 'a1) cnf **)
 
-let qnegate t0 tg =
-  cnf_negate { qnum = Z0; qden = XH } { qnum = (Zpos XH); qden = XH } qplus
-    qmult qminus qopp qeq_bool qle_bool t0 tg
+let qnegate _ =
+  cnf_negate { qnum = Z0; qden = XH } { qnum = (Zpos XH); qden = XH } qplus qmult
+    qminus qopp qeq_bool qle_bool
 
 (** val qunsat : q nFormula -> bool **)
 
@@ -2421,15 +2385,15 @@ let qdeduce =
 (** val normQ : q pExpr -> q pol **)
 
 let normQ =
-  norm { qnum = Z0; qden = XH } { qnum = (Zpos XH); qden = XH } qplus qmult
-    qminus qopp qeq_bool
+  norm { qnum = Z0; qden = XH } { qnum = (Zpos XH); qden = XH } qplus qmult qminus
+    qopp qeq_bool
 
 (** val cnfQ :
-    kind -> (q formula, 'a1, 'a2, 'a3) tFormula -> (q nFormula, 'a1)
-    cnf * 'a1 list **)
+    kind -> bool -> (q formula, 'a1, 'a2, 'a3) tFormula -> (q nFormula, 'a1) cnf * 'a1
+    list **)
 
-let cnfQ k f =
-  rxcnf qunsat qdeduce qnormalise qnegate true k f
+let cnfQ k b f =
+  rxcnf qunsat qdeduce qnormalise qnegate b k f
 
 (** val qTautoChecker : q formula bFormula -> qWitness list -> bool **)
 
@@ -2474,20 +2438,32 @@ type rWitness = q psatz
 (** val rWeakChecker : q nFormula list -> q psatz -> bool **)
 
 let rWeakChecker =
-  check_normalised_formulas { qnum = Z0; qden = XH } { qnum = (Zpos XH);
-    qden = XH } qplus qmult qeq_bool qle_bool
+  check_normalised_formulas { qnum = Z0; qden = XH } { qnum = (Zpos XH); qden = XH }
+    qplus qmult qeq_bool qle_bool
 
 (** val rnormalise : q formula -> 'a1 -> (q nFormula, 'a1) cnf **)
 
 let rnormalise t0 tg =
-  cnf_normalise { qnum = Z0; qden = XH } { qnum = (Zpos XH); qden = XH }
-    qplus qmult qminus qopp qeq_bool qle_bool t0 tg
+  cnf_normalise { qnum = Z0; qden = XH } { qnum = (Zpos XH); qden = XH } qplus qmult
+    qminus qopp qeq_bool qle_bool t0 tg
+
+(** val rnormalise_kind : kind -> q formula -> 'a1 -> (q nFormula, 'a1) cnf **)
+
+let rnormalise_kind = function
+| IsProp -> rnormalise
+| IsBool -> (fun _ _ -> []::[])
 
 (** val rnegate : q formula -> 'a1 -> (q nFormula, 'a1) cnf **)
 
 let rnegate t0 tg =
-  cnf_negate { qnum = Z0; qden = XH } { qnum = (Zpos XH); qden = XH } qplus
-    qmult qminus qopp qeq_bool qle_bool t0 tg
+  cnf_negate { qnum = Z0; qden = XH } { qnum = (Zpos XH); qden = XH } qplus qmult
+    qminus qopp qeq_bool qle_bool t0 tg
+
+(** val rnegate_kind : kind -> q formula -> 'a1 -> (q nFormula, 'a1) cnf **)
+
+let rnegate_kind = function
+| IsProp -> rnegate
+| IsBool -> (fun _ _ -> []::[])
 
 (** val runsat : q nFormula -> bool **)
 
@@ -2502,6 +2478,5 @@ let rdeduce =
 (** val rTautoChecker : rcst formula bFormula -> rWitness list -> bool **)
 
 let rTautoChecker f w =
-  tauto_checker runsat rdeduce rnormalise rnegate (fun cl ->
-    rWeakChecker (map fst cl))
-    (map_bformula IsProp (map_Formula q_of_Rcst) f) w
+  tauto_checker runsat rdeduce rnormalise_kind rnegate_kind (fun cl ->
+    rWeakChecker (map fst cl)) (map_bformula IsProp (map_Formula q_of_Rcst) f) w
